\documentclass[a4paper,11pt]{article}

% Page setup
\usepackage[a4paper,margin=2.5cm]{geometry}

% Fonts & encoding
\usepackage[utf8]{inputenc}
\usepackage[T1]{fontenc}
\usepackage[english]{babel}

% Math
\usepackage{amsmath, amssymb, amsthm}

% Graphics
\usepackage{graphicx}

% Hyperlinks
\usepackage[colorlinks=true,linkcolor=blue,urlcolor=blue,citecolor=blue]{hyperref}

% Optional: numbered equations only if referenced
%\usepackage{mathtools}
%\mathtoolsset{showonlyrefs}

\usepackage{amsmath, amssymb, amsthm}
\usepackage{braket}   % Convenient Dirac notation


\title{Sample Document with Equations}
\author{Your Name}
\date{\today}

\begin{document}

\tableofcontents

\section{Equations}


\subsection*{Slide 5}

\begin{equation}
\hat{H} = \hat{K} + g\hat{V}
\end{equation}


\subsection*{Slide 6}
\addcontentsline{toc}{subsection}{Slide 6}

\begin{align}
  \hat{H} &= \sum_{x}\sum_{p, p'} h^{p}_{p'}(x) \hat{e}^{p}_{p'}(x) + g \sum_{x \ne y}\sum_{p, p', q, q'} V^{pq}_{p'q'}(x, y) \hat{e}^{p}_{p'}(x) \hat{e}^{q}_{q'}(y) \\
  &\equiv \sum_{x}\sum_{p, p'} \hat{h}^{p}_{p'}(x) + g \sum_{x \ne y}\sum_{p, p', q, q'} \hat{V}^{pq}_{p'q'}(x, y) \\
\end{align}

\begin{equation}
  \hat{e}^{p}_{p'}(x) = \ket{p}\bra{p'}(x)
\end{equation}

\begin{equation}
  \hat{e}(x) = (cos(\varphi), sin(\varphi))
\end{equation}

\begin{equation}
\hat{H} = \sum_{i=1}^{N} \hat{h}_{i} + g \sum_{i=1}^{N-1} [\hat{e}_{i}\hat{e}_{i+1} + g(1-3\cos\gamma)(\hat{e}_{i}\hat{r})(\hat{e}_{i+1}\hat{r})]
\end{equation}

\begin{equation}
  \langle p, q \vert \hat{V} \vert p', q' \rangle
\end{equation}

\begin{equation}
  \lvert p - q \rvert = \lvert p' - q' \rvert = 1
\end{equation}


\subsection*{Slide 7}
\addcontentsline{toc}{subsection}{Slide 7}

\begin{equation}
\dim(\hat H) = N \times N
\end{equation}

\begin{equation}
N = \mathrm{state}^{\mathrm{site}}
\end{equation}


\subsection*{Slide 8}
\addcontentsline{toc}{subsection}{Slide 8}

\begin{equation}
M_{dense}(state^{site}) = \frac{8 \,\bigl(\mathrm{state}^{\mathrm{site}}\bigr)^{2}}{1024^{3}}
\end{equation}

\begin{equation}
M_{sparse}(state^{site}) = \frac{24(2state - 2)^{2} state^{site - 2}}{1024^{3}}
\end{equation}

\begin{equation}
M_{dense}(state^{site}) \approx state^{2 \times site}
\end{equation}

\begin{equation}
M_{sparse}(state^{site}) \approx state^{site - 2}
\end{equation}


\subsection*{Slide 9}
\addcontentsline{toc}{subsection}{Slide 9}

\begin{equation}
    \phi : M \longrightarrow P, \qquad
    \phi(m) =
    \begin{cases}
    \text{2|m +1| +1}, & m<0\\[6pt]
    \text{2m}, & m\ge 0
    \end{cases}
\end{equation}

\begin{equation}
M = \{-n,\dots,n\}, \quad
P = \{0,\dots,2n\} \;(\text{so } N=2n)
\end{equation}

\begin{align}
  \braket{\lambda, p', \mu|h|\lambda, p, \mu} &= \hat{h}^{p}_{p'} \\
  \braket{\lambda, p', \nu, q', \mu|V|\lambda, p, \nu, q, \mu} &= \hat{V}^{pq}_{p'q'} \\
\end{align}


\subsection*{Slide 10}
\addcontentsline{toc}{subsection}{Slide 10}

\begin{align}
  \hat{H} &= \sum_{x}\sum_{p, p'} h^{p}_{p'}(x) \hat{e}^{p}_{p'}(x) + g \sum_{x \ne y}\sum_{p, p', q, q'} V^{pq}_{p'q'}(x, y) \hat{e}^{p}_{p'}(x) \hat{e}^{q}_{q'}(y) \\
  &\equiv \sum_{x}\sum_{p, p'} \hat{h}^{p}_{p'}(x) + g \sum_{x \ne y}\sum_{p, p', q, q'} \hat{V}^{pq}_{p'q'}(x, y) \\
\end{align}


\subsection*{Slide 12}
\addcontentsline{toc}{subsection}{Slide 12}

\begin{equation}
\hat{D}_{1} = D^{p}_{p'} = \sum_{\lambda, \mu} C^*_{(\lambda, p, \mu)} C_{(\lambda, p', \mu)}
\end{equation}

\begin{equation}
\hat{D}_{1}\boldsymbol{\psi}_{i} = N_{i}\boldsymbol{\psi}_{i}, \qquad 0\le N_{i}\le 1
\end{equation}

\begin{equation}
f : \mathbb{R} \longrightarrow \mathbb{R}, \qquad f(x)=x^2
\end{equation}

\begin{equation}
U_{NO} = \bigl[\,\boldsymbol{\psi}_1\;\boldsymbol{\psi}_2\;\cdots\;\boldsymbol{\psi}_n\,\bigr]
\end{equation}

\begin{align}
\boldsymbol{\hat{h}} &= U_{NO}^{\dagger} \cdot \hat{V} \cdot U_{NO} \\
\boldsymbol{\hat{V}} &= (U_{NO} \otimes U_{NO})^{\dagger} \cdot \hat{V} \cdot (U_{NO} \otimes U_{NO}) \\
\boldsymbol{\hat{H}} &= \sum_{x}\sum_{p, p'} \boldsymbol{\hat{h}}^{p}_{p'}(x) + g \sum_{x<y}\sum_{p, p', q, q'} \boldsymbol{\hat{V}}^{pq}_{p'q'}(x, y) \\
\end{align}


\subsection*{Slide 14}
\addcontentsline{toc}{subsection}{Slide 14}

\begin{equation}
\hat{D}_{1} = D^{p}_{p'} = \sum_{\lambda, \mu} C^*_{(\lambda, p, \mu)} C_{(\lambda, p', \mu)}
\end{equation}

\begin{equation}
\lambda_1, \lambda_2 \approx 0.495081, 0.495081
\end{equation}

\begin{equation}
\mathbf{v}_1 =
\begin{pmatrix}
-9.770\times 10^{-1} \\
 0 \\
 0 \\
 1.507\times 10^{-1} \\
 1.507\times 10^{-1} \\
 0 \\
 0 \\
-1.727\times 10^{-3} \\
-1.727\times 10^{-3} \\
 0 \\
 0
\end{pmatrix},
\quad
\mathbf{v}_2 =
\begin{pmatrix}
 0 \\
-8.765\times 10^{-4} \\
 8.765\times 10^{-4} \\
 0 \\
 0 \\
 3.192\times 10^{-5} \\
-3.192\times 10^{-5} \\
 0 \\
 0 \\
-1.509\times 10^{-7} \\
 1.509\times 10^{-7}
\end{pmatrix}.
\end{equation}

\subsection*{Slide 20}
\addcontentsline{toc}{subsection}{Slide 20}

\begin{equation}
(-1) \frac{d}{d \tau} \ket{\Psi(\tau)}= \hat{H}\ket{\boldmath{\Psi}(\tau)}
\end{equation}

\begin{equation}
\ket{\Psi(\tau)}= e^{\hat{T}(\tau)}\ket{0}
\end{equation}

\begin{equation}
(-1) \frac{d t_{\lambda}}{d \tau}= R_{\lambda}
\end{equation}


\subsection*{Slide 22}
\addcontentsline{toc}{subsection}{Slide 22}

\begin{align}
\hat{h}^{p}_{p'}(0)  &= \hat{h}^{p}_{p'}(x)  \qquad 0\le x \le N_{sites} \\
\hat{V}^{pq}_{p'q'}(0, 1) &= \hat{V}^{pq}_{p'q'}(x, x+1)  \qquad 0\le x \le N_{sites} - 1 \\
\hat{V}^{pq}_{p'q'}(x, y) &= \hat{V}^{pq}_{p'q'}(y, x)  \qquad 0\le x, y \le N_{sites}, |x - y| = 1 \\
\end{align}

\begin{align}
  Rt^{ab}_{ij}(x < y) &= Rs^{ab}_{ij}(x< y) + Rn^{ab}_{ij}(x, y) + Rn^{ab}_{ij}(y, x) \\
  &= Rs^{ab}_{ij}(x< y) + 2 \times Rn^{ab}_{ij}(x, y) \\
\end{align}


\subsection*{Slide 22}
\addcontentsline{toc}{subsection}{Slide 22}

\begin{equation}
D(\mathrm{state},\mathrm{site}) = \frac{E_{\mathrm{state}}}{E_{\mathrm{site}}}
= \frac{\mathrm{site}}{\ln(\mathrm{state})}.
\end{equation}


\subsection*{Slide 24}
\addcontentsline{toc}{subsection}{Slide 24}

\begin{equation*}
A^{a}_{p}(x)\,A^{b}_{q}(y)\,V^{pq}_{cd}(x,y)\,t^{cd}_{ij}(x,y)
\;\longrightarrow\;
A^{a}_{p}(x)\,A^{b}_{q}(y)\,V^{pq}_{cd}(x,y)\,t^{cd}_{\boldsymbol{\cdot} \ \boldsymbol{\cdot}}(x,y)
\;\longrightarrow\;
A A^{B=ab}_{Q=pq}(x,y)\,V^{Q}_{C}(x,y)\,t^{C}_{\ \boldsymbol{\cdot}}(x,y)
\end{equation*}

\end{document}
